Compile.v
@@ -1,0 +1,75 @@
+(** This is the top level driver for the compiler. *)
+
+From Coq Require Import String List ListSet Arith NArith.
+From Vyper Require Import Config Calldag.
+From Vyper.L10 Require AST Callset Descend Interpret.
+From Vyper.From10To20 Require FunCtx Call.
+From Vyper.From20To30 Require FunCtx Call.
+From Vyper Require Import ConstFold L10.Base.
+
+(** This is the verified part of the compiler.
+    This function translates a L10 calldag into a L30 calldag (or an error).
+ *)
+Definition translate_10_to_30 {C: VyperConfig} (calldag10: L10.Descend.calldag)
+: string + L30.Descend.calldag
+:= let calldag20 := From10To20.FunCtx.translate_calldag calldag10 (* no errors possible *) in
+   match const_fold_calldag calldag20 with
+   | inl err => inl err
+   | inr calldag20' => From20To30.FunCtx.translate_calldag calldag20'
+   end.
+
+(** This is the theorem verifying that the compiler works as intended.
+ *)
+Theorem translate_10_to_30_ok {C: VyperConfig}
+                              (calldag10: L10.Descend.calldag)
+                              (calldag30: L30.Descend.calldag)
+                              (ok: translate_10_to_30 calldag10 = inr calldag30)
+                              (builtins: string -> option builtin)
+                              (fun_name: string)
+                              (world: world_state)
+                              (arg_values: list uint256):
+  L30.Interpret.interpret builtins calldag30 fun_name world arg_values
+   =
+  L10.Interpret.interpret builtins calldag10 fun_name world arg_values.
+Proof.
+(* 10 -> 20 *)
+rewrite<- From10To20.Call.translate_ok.
+unfold translate_10_to_30 in ok.
+remember (From10To20.FunCtx.translate_calldag calldag10) as calldag20.
+clear Heqcalldag20.
+
+(* const fold *)
+remember (const_fold_calldag calldag20) as calldag20'. symmetry in Heqcalldag20'.
+destruct calldag20' as [|calldag20']. { discriminate. }
+rewrite<- (const_fold_ok _ Heqcalldag20').
+clear Heqcalldag20'.
+
+(* 20 -> 30 *)
+apply From20To30.Call.translate_ok. exact ok.
+Qed.
+
+(** This function takes the parser output, which is a list of L10 declarations,
+    and compiles it into a L30 calldag.
+
+    Here [make_calldag] converts the output of the parser to the input to the verified compiler.
+ *)
+Definition compile_to_L30 {C: VyperConfig} (parsed_src: list L10.AST.decl)
+: string + L30.Descend.calldag
+:= match make_calldag L10.AST.decl_name L10.Callset.decl_callset parsed_src with
+   | inl err => inl err
+   | inr cd => translate_10_to_30 cd
+   end.
+
+Definition calldag_to_string {C: VyperConfig} (cd: L30.Descend.calldag)
+:= let _ := string_map_impl in
+   (List.fold_right (fun x tail => x ++ L10.ToString.newline ++ tail) ""
+                    (List.map (fun kv => (L30.AST.string_of_decl (snd kv))) 
+                              (Map.items (cd_decls cd))))%string.
+
+(** This is the compiler without parser. *)
+Definition compile {C: VyperConfig} (parsed_src: list L10.AST.decl)
+: string + string
+:= match compile_to_L30 parsed_src with
+   | inl err => inl err
+   | inr cd => inr (calldag_to_string cd)
+   end.
