Extract.v
@@ -1,12 +1,16 @@
-From Coq Require Import ExtrOcamlBasic ExtrOcamlString ExtrHaskellBasic ExtrHaskellString.
-From Vyper Require Import Config L10.AST From20To30.Translate.
+From Coq Require Import ExtrOcamlBasic ExtrOcamlString.
+From Coq Require Import ExtrHaskellBasic ExtrHaskellString.
+From Vyper Require Import L10.AST Config Compile.
 
 Extraction Language Haskell.
 
 Extraction "haskell/Extracted.hs"
-  L10.AST.unop
-  L10.AST.binop (* this is to prevent [comparison] from taking [Lt], [Gt] and [Eq] *)
-  L10.AST.decl
-  translate_decl
+  L10.AST.BinopLt
+  L10.AST.BinopGt
+  L10.AST.BinopEq
+  L10.AST.BinopLe
+  L10.AST.BinopGe
+  L10.AST.BinopNe
+  compile
   uint256_of_Z
   sample_config.
