L10/AST.v
@@ -1,20 +1,10 @@
-From Coq Require Import String List HexString.
-
 Require Import Config FSet.
-
-Local Open Scope string_scope.
+From Coq Require Import String List.
 
 Inductive unop
 := BitwiseNot
  | LogicalNot
  | Neg.
-
-Definition string_of_unop (op: unop)
-:= match op with
-   | LogicalNot => "not"
-   | BitwiseNot => "~"
-   | Neg => "-"
-   end.
 
 Inductive binop
 := (* LogicalOr
@@ -42,39 +32,20 @@ Inductive binop
  | Mod
  | Pow.
 
-
-Definition string_of_binop (op: binop)
-:= match op with
-   | Lt => "<"
-   | Le => "<="
-   | Gt => ">"
-   | Ge => ">="
-   | Eq => "=="
-   | Ne => "!="
-   | BitwiseOr  => "|"
-   | BitwiseAnd => "&"
-   | BitwiseXor => "^"
-   | ShiftLeft  => "<<"
-   | ShiftRight => ">>"
-   | Add => "+"
-   | Sub => "-"
-   | Mul => "*"
-   | Quot => "//"
-   | Mod => "%"
-   | Pow => "**"
-   end.
-
-
+(** I cannot make the extractor reliably prioritize [binop] over [comparison],
+    resulting in ugly names like [Lt0] for my binops. Here's a workaround that
+    is still ugly but not as much as [Lt0].
+ *)
+Definition BinopLt := Lt.
+Definition BinopGt := Gt.
+Definition BinopEq := Eq.
+Definition BinopLe := Le.
+Definition BinopGe := Le.
+Definition BinopNe := Ne.
 
 Inductive assignable
 := AssignableLocalVar (name: string)
  | AssignableStorageVar (name: string).
-
-Definition string_of_assignable (a: assignable)
-:= match a with
-   | AssignableLocalVar name => name
-   | AssignableStorageVar name => "self." ++ name
-   end.
 
 Section AST.
 
@@ -221,104 +192,5 @@ Next Obligation.
 destruct s; cbn in IsVarDecl; try discriminate.
 assert (Bad := H name init). tauto.
 Qed.
-
-(****************************   format   ******************************)
-
-Fixpoint string_of_expr (e: expr)
-:= match e with
-   | Const u => HexString.of_Z (Z_of_uint256 u)
-   | LocalVar name => name
-   | StorageVar name => "self." ++ name
-   | UnOp op a => "(" ++ string_of_unop op ++ string_of_expr a ++ ")"
-   | BinOp op a b => "(" ++ string_of_expr a ++ " " ++ string_of_binop op
-                         ++ " " ++ string_of_expr b ++ ")"
-   | IfThenElse cond yes no => "(" ++ string_of_expr yes ++ " if "
-                                   ++ string_of_expr cond ++ " else "
-                                   ++ string_of_expr no ++ ")"
-   | LogicalAnd a b => "(" ++ string_of_expr a ++ " and " ++ string_of_expr b ++ ")"
-   | LogicalOr  a b => "(" ++ string_of_expr a ++ " or "  ++ string_of_expr b ++ ")"
-   | PrivateOrBuiltinCall name args => name ++ "(" ++
-       (let fix string_of_expr_list_with_preceding_commas {C: VyperConfig} (a: list expr)
-            := fold_right (fun e tail => ", " ++ string_of_expr e ++ tail) "" a
-        in match args with
-           | nil => ""
-           | h :: t => string_of_expr h ++
-                         string_of_expr_list_with_preceding_commas t
-           end) ++ ")"
-   end.
-
-
-Fixpoint string_of_small_stmt {C: VyperConfig} (ss: small_stmt)
-:= match ss with
-   | Pass => "pass"
-   | Break => "break"
-   | Continue => "continue"
-   | Return None => "return"
-   | Return (Some e) => "return " ++ string_of_expr e
-   | Revert => "revert"
-   | Raise err => "raise " ++ string_of_expr err
-   | Assert cond None => "assert " ++ string_of_expr cond
-   | Assert cond (Some err) => "assert " ++ string_of_expr cond ++ ", " ++ string_of_expr err
-   | Assign lhs rhs => string_of_assignable lhs ++ " = " ++ string_of_expr rhs
-   | BinOpAssign lhs op rhs => string_of_assignable lhs ++ " "
-                            ++ string_of_binop op ++ "= " ++ string_of_expr rhs
-   | ExprStmt e => string_of_expr e
-   end.
-
-Definition add_indent (lines: list string)
-:= map (fun s => "    " ++ s) lines.
-
-Definition newline := "
-".
-
-Fixpoint lines_of_stmt (s: stmt)
-: list string
-:= let fix lines_of_stmt_list (l: list stmt)
-       := match l with
-          | nil => nil
-          | h :: t => (lines_of_stmt h ++ lines_of_stmt_list t)%list
-          end
-   in match s with
-      | SmallStmt ss => string_of_small_stmt ss :: nil
-      | LocalVarDecl name None => ("var " ++ name) :: nil
-      | LocalVarDecl name (Some init) => ("var " ++ name ++ " = " ++ string_of_expr init) :: nil
-      | IfElseStmt cond yes None => ("if " ++ string_of_expr cond ++ ":") 
-                                    :: add_indent (lines_of_stmt_list yes)
-      | IfElseStmt cond yes (Some no) => ("if " ++ string_of_expr cond ++ ":")
-                                          :: add_indent (lines_of_stmt_list yes)
-                                          ++ "else:" :: add_indent (lines_of_stmt_list no)
-      | FixedRangeLoop name None stop body => ("for " ++ name ++ " in range("
-                                               ++ HexString.of_Z (Z_of_uint256 stop) ++ "):")
-                                               :: add_indent (lines_of_stmt_list body)
-      | FixedRangeLoop name (Some start) stop body => ("for " ++ name ++ " in range("
-                                                     ++ HexString.of_Z (Z_of_uint256 start) ++ ", "
-                                                     ++ HexString.of_Z (Z_of_uint256 stop) ++ "):")
-                                                     :: add_indent (lines_of_stmt_list body)
-      | FixedCountLoop name start count body =>  ("for " ++ name ++ " in count("
-                                                     ++ string_of_expr start ++ ", "
-                                                     ++ HexString.of_Z (Z_of_uint256 count) ++ "):")
-                                                     :: add_indent (lines_of_stmt_list body)
-      end.
-
-Fixpoint lines_of_stmt_list (l: list stmt)
-:= match l with
-   | nil => nil
-   | h :: t => (lines_of_stmt h ++ lines_of_stmt_list t)%list
-   end.
-
-Definition lines_of_decl (d: decl)
-:= match d with
-   | StorageVarDecl name => ("var " ++ name) :: nil
-   | FunDecl name args body =>
-       ("def " ++ name ++ "(" ++
-         match args with
-         | nil => ""
-         | h :: t => h ++ fold_right (fun x tail => ", " ++ x ++ tail) "" t
-         end ++ "):")
-       :: add_indent (lines_of_stmt_list body)
-   end.
-
-Definition string_of_decl {C: VyperConfig} (d: decl)
-:= newline ++ fold_right (fun x tail => x ++ newline ++ tail) "" (lines_of_decl d).
 
 End AST.
