L10/ToString.v
@@ -1,0 +1,143 @@
+From Coq Require Import String List HexString.
+
+Require Import Config FSet.
+
+From Vyper Require Import L10.AST.
+
+Local Open Scope string_scope.
+
+Definition string_of_unop (op: unop)
+:= match op with
+   | LogicalNot => "not"
+   | BitwiseNot => "~"
+   | Neg => "-"
+   end.
+
+Definition string_of_binop (op: binop)
+:= match op with
+   | Lt => "<"
+   | Le => "<="
+   | Gt => ">"
+   | Ge => ">="
+   | Eq => "=="
+   | Ne => "!="
+   | BitwiseOr  => "|"
+   | BitwiseAnd => "&"
+   | BitwiseXor => "^"
+   | ShiftLeft  => "<<"
+   | ShiftRight => ">>"
+   | Add => "+"
+   | Sub => "-"
+   | Mul => "*"
+   | Quot => "//"
+   | Mod => "%"
+   | Pow => "**"
+   end.
+
+
+Definition string_of_assignable (a: assignable)
+:= match a with
+   | AssignableLocalVar name => name
+   | AssignableStorageVar name => "self." ++ name
+   end.
+
+
+(****************************   format   ******************************)
+
+Fixpoint string_of_expr {C: VyperConfig} (e: expr)
+:= match e with
+   | Const u => HexString.of_Z (Z_of_uint256 u)
+   | LocalVar name => name
+   | StorageVar name => "self." ++ name
+   | UnOp op a => "(" ++ string_of_unop op ++ string_of_expr a ++ ")"
+   | BinOp op a b => "(" ++ string_of_expr a ++ " " ++ string_of_binop op
+                         ++ " " ++ string_of_expr b ++ ")"
+   | IfThenElse cond yes no => "(" ++ string_of_expr yes ++ " if "
+                                   ++ string_of_expr cond ++ " else "
+                                   ++ string_of_expr no ++ ")"
+   | LogicalAnd a b => "(" ++ string_of_expr a ++ " and " ++ string_of_expr b ++ ")"
+   | LogicalOr  a b => "(" ++ string_of_expr a ++ " or "  ++ string_of_expr b ++ ")"
+   | PrivateOrBuiltinCall name args => name ++ "(" ++
+       (let fix string_of_expr_list_with_preceding_commas {C: VyperConfig} (a: list expr)
+            := fold_right (fun e tail => ", " ++ string_of_expr e ++ tail) "" a
+        in match args with
+           | nil => ""
+           | h :: t => string_of_expr h ++
+                         string_of_expr_list_with_preceding_commas t
+           end) ++ ")"
+   end.
+
+
+Fixpoint string_of_small_stmt {C: VyperConfig} (ss: small_stmt)
+:= match ss with
+   | Pass => "pass"
+   | Break => "break"
+   | Continue => "continue"
+   | Return None => "return"
+   | Return (Some e) => "return " ++ string_of_expr e
+   | Revert => "revert"
+   | Raise err => "raise " ++ string_of_expr err
+   | Assert cond None => "assert " ++ string_of_expr cond
+   | Assert cond (Some err) => "assert " ++ string_of_expr cond ++ ", " ++ string_of_expr err
+   | Assign lhs rhs => string_of_assignable lhs ++ " = " ++ string_of_expr rhs
+   | BinOpAssign lhs op rhs => string_of_assignable lhs ++ " "
+                            ++ string_of_binop op ++ "= " ++ string_of_expr rhs
+   | ExprStmt e => string_of_expr e
+   end.
+
+Definition add_indent {C: VyperConfig} (lines: list string)
+:= map (fun s => "    " ++ s) lines.
+
+Definition newline := "
+".
+
+Fixpoint lines_of_stmt {C: VyperConfig} (s: stmt)
+: list string
+:= let fix lines_of_stmt_list (l: list stmt)
+       := match l with
+          | nil => nil
+          | h :: t => (lines_of_stmt h ++ lines_of_stmt_list t)%list
+          end
+   in match s with
+      | SmallStmt ss => string_of_small_stmt ss :: nil
+      | LocalVarDecl name None => ("var " ++ name) :: nil
+      | LocalVarDecl name (Some init) => ("var " ++ name ++ " = " ++ string_of_expr init) :: nil
+      | IfElseStmt cond yes None => ("if " ++ string_of_expr cond ++ ":") 
+                                    :: add_indent (lines_of_stmt_list yes)
+      | IfElseStmt cond yes (Some no) => ("if " ++ string_of_expr cond ++ ":")
+                                          :: add_indent (lines_of_stmt_list yes)
+                                          ++ "else:" :: add_indent (lines_of_stmt_list no)
+      | FixedRangeLoop name None stop body => ("for " ++ name ++ " in range("
+                                               ++ HexString.of_Z (Z_of_uint256 stop) ++ "):")
+                                               :: add_indent (lines_of_stmt_list body)
+      | FixedRangeLoop name (Some start) stop body => ("for " ++ name ++ " in range("
+                                                     ++ HexString.of_Z (Z_of_uint256 start) ++ ", "
+                                                     ++ HexString.of_Z (Z_of_uint256 stop) ++ "):")
+                                                     :: add_indent (lines_of_stmt_list body)
+      | FixedCountLoop name start count body =>  ("for " ++ name ++ " in count("
+                                                     ++ string_of_expr start ++ ", "
+                                                     ++ HexString.of_Z (Z_of_uint256 count) ++ "):")
+                                                     :: add_indent (lines_of_stmt_list body)
+      end.
+
+Fixpoint lines_of_stmt_list {C: VyperConfig} (l: list stmt)
+:= match l with
+   | nil => nil
+   | h :: t => (lines_of_stmt h ++ lines_of_stmt_list t)%list
+   end.
+
+Definition lines_of_decl {C: VyperConfig} (d: decl)
+:= match d with
+   | StorageVarDecl name => ("var " ++ name) :: nil
+   | FunDecl name args body =>
+       ("def " ++ name ++ "(" ++
+         match args with
+         | nil => ""
+         | h :: t => h ++ fold_right (fun x tail => ", " ++ x ++ tail) "" t
+         end ++ "):")
+       :: add_indent (lines_of_stmt_list body)
+   end.
+
+Definition string_of_decl {C: VyperConfig} (d: decl)
+:= newline ++ fold_right (fun x tail => x ++ newline ++ tail) "" (lines_of_decl d).
+
